switching asm.fst to --universes ... cleaner and composing blocks works

examples/asm/asm.fst
@@ -2,64 +2,66 @@ module Asm
 
 type reg = int
 
-kind ASM_Pre = STPre_h reg
-kind ASM_Post (a:Type) = STPost_h reg a
-kind ASM_WP (a:Type) = STWP_h reg a
+let asm_pre = st_pre_h reg
+let asm_post a = st_post_h reg a
+let asm_wp a = st_wp_h reg a
 
 new_effect ASM_ = STATE_h reg //the effect ASM is very primitive, we won't use it much in specs
 sub_effect
-  DIV   ~> ASM_ = fun (a:Type) (wp:PureWP a) (p:ASM_Post a) (r:reg) -> wp (fun a -> p a r)
+  DIV   ~> ASM_ = fun (a:Type) (wp:pure_wp a) (p:asm_post a) (r:reg) -> wp (fun a -> p a r)
 
 
-effect ASM (a:Type) (wp:ASM_WP a) = ASM_ a wp wp  //we'll use this one instead
-effect Asm (a:Type) (pre:ASM_Pre) (post: (reg -> ASM_Post a)) = //and this one, which is more like a Hoare triple
+effect ASM (a:Type) (wp:asm_wp a) = ASM_ a wp wp  //we'll use this one instead
+effect Asm (a:Type) (pre:asm_pre) (post: (reg -> Tot (asm_post a))) = //and this one, which is more like a Hoare triple
        ASM_ a
-             (fun (p:ASM_Post a) (h:reg) -> pre h /\ (forall a h1. (pre h /\ post h a h1) ==> p a h1)) (* WP *)
-             (fun (p:ASM_Post a) (h:reg) -> pre h /\ (forall a h1. (pre h /\ post h a h1) ==> p a h1)) (* WP *)
-             (* (fun (p:ASM_Post a) (h:reg) -> (forall a h1. (pre h /\ post h a h1) ==> p a h1))         (\* WLP *\) *)
+             (fun (p:asm_post a) (h:reg) -> pre h /\ (forall a h1. (pre h /\ post h a h1) ==> p a h1)) (* WP *)
+             (fun (p:asm_post a) (h:reg) -> pre h /\ (forall a h1. (pre h /\ post h a h1) ==> p a h1)) (* WP *)
+             (* (fun (p:asm_post a) (h:reg) -> (forall a h1. (pre h /\ post h a h1) ==> p a h1))         (\* WLP *\) *)
 
 
-type instr = 
+type instr =
   | Add : int -> instr
   | Sub : int -> instr
 
 val eval : instr -> reg -> Tot reg
-let eval i r = match i with 
+let eval i r = match i with
   | Add j -> r + j
   | Sub j -> r - j
 
 
 type prog = list instr
 
-val finished : unit -> ASM prog  (fun (post:ASM_Post prog) (r0:reg) -> post [] r0)
+val finished : unit -> ASM prog  (fun post r0 -> post [] r0)
 let finished _ = []
 
-val nop : unit -> ASM prog  (fun (post:ASM_Post prog) (r0:reg) -> post [] r0)
+val nop : unit -> ASM prog  (fun post r0 -> post [] r0)
 let nop _ = []
 
 
-type ASMComp (wp:ASM_WP prog) = unit -> ASM prog wp
-type AsmComp (pre:ASM_Pre) (post:reg -> ASM_Post prog) = unit -> Asm prog pre post
+type ASMComp wp = unit -> ASM prog wp
+type AsmComp pre post = = unit -> Asm prog pre post
 
-assume val op_Hat_Hat : #wp:ASM_WP prog
-	       -> i:instr 
+assume val op_Hat_Hat : #wp:asm_wp prog
+	       -> i:instr
 	       -> =f:ASMComp wp
-	       -> Tot (ASMComp (fun (post:ASM_Post prog) (r0:reg) -> 
+	       -> Tot (ASMComp (fun post r0 -> 
 			      wp (fun p r1 -> post (i::p) r1) (eval i r0)))
 
 val add_2: AsmComp (requires (fun r -> True))
 		  (ensures (fun r_0 p r_1 -> r_1 = r_0 + 2))
 let add_2 =  //^^ associates the wrong way, unfortunately
-       (Add 1  
+       (Add 1
     ^^ (Add 1
     ^^ finished))
 
-//we could define an operator that sequences in the other direction, a snoc instead of a cons
-assume val op_Hat_Bar : #wp:ASM_WP prog
+assume val append : list 'a -> list 'a -> Tot (list 'a)
+
+//we could define an operator that sequences in the other direction, a snoc instead of a cons 
+assume val op_Hat_Bar : #wp:asm_wp prog
 	       -> =f:ASMComp wp
-      	       -> i:instr 
-	       -> Tot (ASMComp (fun (post:ASM_Post prog) (r0:reg) -> 
-			      wp (fun p r1 -> post (List.append p [i]) (eval i r1)) r0))
+      	       -> i:instr
+	       -> Tot (ASMComp (fun post r0 -> 
+			      wp (fun p r1 -> post (append p [i]) (eval i r1)) r0))
 val add_3: AsmComp (requires (fun r -> True))
 		  (ensures (fun r_0 p r_1 -> r_1 = r_0 + 3))
 let add_3 = nop
@@ -68,7 +70,7 @@ let add_3 = nop
     ^| (Add 1)
 
 
-val add_4: AsmComp 
+val add_4: AsmComp
   (requires (fun r -> True))
   (ensures (fun r_0 p r_1 -> r_1 = r_0 + 4))
 let add_4 = nop
@@ -78,16 +80,15 @@ let add_4 = nop
   ^| (Sub 2)
 
 (* Composing two basic blocks in sequence *)
-assume val op_Hat_Hat_Hat : 
-          #wp1:ASM_WP prog
-	-> #wp2:ASM_WP prog
+assume val op_Hat_Hat_Hat :
+          #wp1:asm_wp prog
+	-> #wp2:asm_wp prog
         -> =f:ASMComp wp1
 	-> =g:ASMComp wp2
-	-> Tot (ASMComp (fun (post:ASM_Post prog) (r0:reg) -> 
-	       wp1 (fun p1 r1 -> 
-	       wp2 (fun p2 r2 -> post (List.append p1 p2) r2) r1) r0))
-
-val add_4': AsmComp 
+	-> Tot (ASMComp (fun (post:asm_post prog) (r0:reg) ->
+	       wp1 (fun p1 r1 ->
+	       wp2 (fun p2 r2 -> post (append p1 p2) r2) r1) r0))
+val add_4': AsmComp
   (requires (fun r -> True))
   (ensures (fun r_0 p r_1 -> r_1 = r_0 + 4))
-(* let add_4' = add_2 ^^^ add_2 //NS: type inference for this one doesn't quite work for some silly reason ... it will once I fix it. *)
+let add_4' = add_2 ^^^ add_2
